Work on boardroom voting

execution/theories/BoardroomVoting.v
@@ -1,13 +1,19 @@
 From Coq Require Import List.
 From Coq Require Import Morphisms.
 From Coq Require Import ZArith.
+From Coq Require Import Znumtheory.
 From Coq Require Import Permutation.
-From Coq Require VectorDef.
+From Coq Require Import Psatz.
+From Coq Require Program.
 From RecordUpdate Require Import RecordUpdate.
 Require Import Automation.
 Require Import Blockchain.
+Require Import BoundedN.
 Require Import Containers.
+From stdpp Require countable.
 Require ContractMonads.
+Require Import Extras.
+Require Import ModularArith.
 Require Import Monads.
 Require Import Serializable.
 
@@ -16,13 +22,26 @@ Import RecordSetNotations.
 
 Section BoardroomVoting.
 Context `{Base : ChainBase}.
-Context `{H : Z -> Z}.
+Context `(H : Z -> Z).
+(*Context (verify_vote (vote : Z) (rk : Z) (jj*)
+Context (modulus : Z).
+Context (generator : Z).
+Context (modulus_prime : prime modulus).
+
+Class VoteProofScheme :=
+  build_vote_proof_scheme {
+    make_vote_proof (pks : list Z) (index : nat)
+                    (secret_key : Z) (secret_vote : bool) : Z;
+    verify_vote (pks : list Z) (index : nat) (public_vote proof : Z) : bool;
+
+    verify_vote_spec pks index pv proof :
+      verify_vote pks index pv proof = true ->
+      exists sk sv, proof = make_vote_proof pks index sk sv;
+  }.
+
+Context `{VoteProofScheme}.
 
 Local Open Scope Z.
-Definition prime : Z :=
-  32317006071311007300338913926423828248817941241140239112842009751400741706634354222619689417363569347117901737909704191754605873209195028853758986185622153212175412514901774520270235796078236248884246189477587641105928646099411723245426622522193230540919037680524235519125679715870117001058055877651038861847280257976054903569732561526167081339361799541336476559160368317896729073178384589680639671900977202194168647225871031411336429319536193471636533209717077448227988588565369208645296636077250268955505928362751121174096972998068410554359584866583291642136218231078990999448652468262416972035911852507045361090559.
-
-Definition generator : Z := 2.
 
 (* Allow us to automatically derive Serializable instances *)
 Set Nonrecursive Elimination Schemes.
@@ -31,7 +50,6 @@ Record Setup :=
   build_setup {
     eligible_voters : FMap Address unit;
     finish_registration_by : nat;
-    begin_election_by : nat;
     finish_commit_by : option nat;
     finish_vote_by : nat;
     registration_deposit : Amount;
@@ -40,7 +58,6 @@ Record Setup :=
 Record VoterInfo :=
   build_voter_info {
     index : nat;
-    public_key : Z;
     vote_hash : Z;
     public_vote : Z;
 }.
@@ -49,6 +66,7 @@ Record State :=
   build_state {
     owner : Address;
     registered_voters : FMap Address VoterInfo;
+    public_keys : list Z;
     setup : Setup;
     result : option nat;
   }.
@@ -56,14 +74,14 @@ Record State :=
 Inductive Msg :=
 | signup (pk : Z)
 | commit_to_vote (hash : Z)
-| submit_vote (v : Z)
+| submit_vote (v : Z) (proof : Z)
 | tally_votes.
 
 Global Instance VoterInfo_settable : Settable _ :=
-  settable! build_voter_info <index; public_key; vote_hash; public_vote>.
+  settable! build_voter_info <index; vote_hash; public_vote>.
 
 Global Instance State_settable : Settable _ :=
-  settable! build_state <owner; registered_voters; setup; result>.
+  settable! build_state <owner; registered_voters; public_keys; setup; result>.
 
 Global Instance Setup_serializable : Serializable Setup :=
   Derive Serializable Setup_rect<build_setup>.
@@ -82,23 +100,16 @@ Import ContractMonads.
 Definition init : ContractIniter Setup State :=
   do owner <- lift caller_addr;
   do setup <- deployment_setup;
+  do lift (if finish_registration_by setup <? finish_vote_by setup then Some tt else None)%nat;
   accept_deployment
     {| owner := owner;
        registered_voters := FMap.empty;
+       public_keys := [];
        setup := setup;
        result := None; |}.
 
-Axiom todo : forall {T}, T.
-
-Definition mod_pow (a x m : Z) : Z := todo.
-
-Lemma mod_pow_spec a x m :
-  mod_pow a x m = a^x mod m.
-Proof.
-  Admitted.
-
 Fixpoint bruteforce_tally (n : nat) (product : Z) : option nat :=
-  if mod_pow generator (Z.of_nat n) prime =? product then
+  if mod_pow generator (Z.of_nat n) modulus =? product then
     Some n
   else
     match n with
@@ -115,12 +126,16 @@ Definition receive : ContractReceiver State Msg State :=
   | signup pk =>
     do lift (if finish_registration_by (setup state) <? cur_slot then None else Some tt)%nat;
     do lift (if FMap.mem caller (eligible_voters (setup state)) then Some tt else None);
-    let index := FMap.size (registered_voters state) in
+    do lift (if FMap.mem caller (registered_voters state) then None else Some tt);
+    do amt <- lift call_amount;
+    do lift (if amt =? (registration_deposit (setup state)) then Some tt else None);
+    let index := length (public_keys state) in
     let inf := {| index := index;
-                  public_key := pk;
                   vote_hash := 0;
                   public_vote := 0; |} in
-    accept_call (state<|registered_voters ::= FMap.add caller inf|>)
+    let new_state := state<|registered_voters ::= FMap.add caller inf|>
+                          <|public_keys ::= fun l => l ++ [pk]|> in
+    accept_call new_state
 
   | commit_to_vote hash =>
     do commit_by <- lift (finish_commit_by (setup state));
@@ -129,10 +144,14 @@ Definition receive : ContractReceiver State Msg State :=
     let inf := inf<|vote_hash := hash|> in
     accept_call (state<|registered_voters ::= FMap.add caller inf|>)
 
-  | submit_vote v =>
+  | submit_vote v proof =>
     do lift (if finish_vote_by (setup state) <? cur_slot then None else Some tt)%nat;
     do inf <- lift (FMap.find caller (registered_voters state));
-    do lift (if H v =? vote_hash inf then Some tt else None);
+    do lift (if finish_commit_by (setup state) then
+               if H v =? vote_hash inf then Some tt else None
+             else
+               Some tt);
+    do lift (if verify_vote (public_keys state) (index inf) v proof then Some tt else None);
     let inf := inf<|public_vote := v|> in
     accept_call (state<|registered_voters ::= FMap.add caller inf|>)
 
@@ -140,7 +159,7 @@ Definition receive : ContractReceiver State Msg State :=
     do lift (if cur_slot <? finish_vote_by (setup state) then None else Some tt)%nat;
     do lift (match result state with | Some _ => None | None => Some tt end);
     let votes := map public_vote (FMap.values (registered_voters state)) in
-    let product := fold_right (fun e r => e * r mod prime) 1%Z votes in
+    let product := fold_right (fun e r => e * r mod modulus) 1%Z votes in
     let max_vote := FMap.size (registered_voters state) in
     do res <- lift (bruteforce_tally max_vote product);
     accept_call (state<|result := Some res|>)
@@ -148,7 +167,11 @@ Definition receive : ContractReceiver State Msg State :=
 
 Program Definition boardroom_voting : Contract Setup Msg State :=
   build_contract init receive _ _.
-Next Obligation. now repeat intro; subst. Qed.
+Next Obligation.
+  repeat intro; subst.
+  cbn -[Nat.ltb].
+  destruct (_ <? _)%nat; auto.
+Qed.
 Next Obligation with cbn -[Nat.leb].
   intros c1 c2 ceq ctx ? <- state ? <- msg ? <-.
   unfold run_contract_receiver...
@@ -157,6 +180,8 @@ Next Obligation with cbn -[Nat.leb].
   - rewrite <- ceq.
     destruct (_ <? _)%nat; auto.
     destruct (FMap.mem _ _); auto.
+    destruct (FMap.mem _ _); auto.
+    destruct (_ =? _)%Z; auto.
   - destruct (finish_commit_by _); auto.
     rewrite <- ceq.
     destruct (_ <? _)%nat; auto.
@@ -164,50 +189,55 @@ Next Obligation with cbn -[Nat.leb].
   - rewrite <- ceq.
     destruct (_ <? _)%nat; auto.
     destruct (FMap.find _ _); auto.
-    destruct (_ =? _); auto.
+    destruct (finish_commit_by _); [destruct (_ =? _); auto|].
+    all: destruct (verify_vote _ _ _ _); auto.
   - rewrite <- ceq.
     destruct (_ <? _)%nat; auto.
     destruct (result _); auto.
     destruct (_ (FMap.size _)); auto.
 Qed.
 
+Definition reconstructed_key (pks : list Z) (n : nat) : Z :=
+  let prod := fold_right (fun e r => (e * r) mod modulus) 1 in
+  let lprod := prod (firstn n pks) in
+  let rprod := mod_inv (prod (skipn (S n) pks)) modulus in
+  (lprod * rprod) mod modulus.
+
+Definition compute_public_key (sk : Z) : Z :=
+  mod_pow generator sk modulus.
+
+Definition compute_public_vote (rk sk : Z) (sv : bool) : Z :=
+  (mod_pow rk sk modulus * if sv then generator else 1) mod modulus.
+
+Definition make_signup_msg (sk : Z) : Msg :=
+  signup (compute_public_key sk).
+
+Definition make_commit_msg (pks : list Z) (my_index : nat) (sk : Z) (sv : bool) : Msg :=
+  commit_to_vote (H (compute_public_vote (reconstructed_key pks my_index) sk sv)).
+
+Definition make_vote_msg (pks : list Z) (my_index : nat) (sk : Z) (sv : bool) : Msg :=
+  submit_vote (compute_public_vote (reconstructed_key pks my_index) sk sv)
+              (make_vote_proof pks my_index sk sv).
+
 Section Theories.
 
-Record PrivateVoterInfo (vinf : VoterInfo) (Yi : Z) :=
-  build_private_voter_info {
-    secret_key : Z;
-    actual_vote : bool;
-    secret_key_match : mod_pow generator secret_key prime = public_key vinf;
-    vote_match :
-      let vote_num := if actual_vote then generator else 1 in
-      public_vote vinf = ((mod_pow Yi secret_key prime) * vote_num) mod prime;
-  }.
-
-(* Find y such that x*y = 1 mod m *)
-Definition mod_inv (x m : Z) : Z := todo.
-Lemma mod_inv_spec x m :
-  (x * mod_inv x m) mod m = 1.
-Proof.
-  Admitted.
-
-Fixpoint reconstructed_keys
-        (voters : list VoterInfo) (cummul : Z) : Vector.t Z (length voters) :=
-  match voters with
-  | [] => Vector.nil
-  | hd :: tl =>
-    let nom := public_key hd * cummul mod prime in
-    let denom := fold_right (fun e r => e * r mod prime) 1 (map public_key voters) in
-    Vector.cons ((nom * mod_inv denom prime) mod prime) (reconstructed_keys tl nom)
+Fixpoint SecretsKnown
+         (sks : Address -> Z)
+         (svs : Address -> bool)
+         (calls : list (ContractCallInfo Msg)) : Prop :=
+  match calls with
+  | call :: calls =>
+    let caller := Blockchain.call_from call in
+    match Blockchain.call_msg call with
+    | Some (signup pk as m) => m = make_signup_msg (sks caller)
+    | Some (submit_vote _ _ as m) =>
+      exists pks my_index, m = make_vote_msg pks my_index (sks caller) (svs caller)
+    | _ => True
+    end /\ SecretsKnown sks svs calls
+  | [] => True
   end.
 
-Definition SecretKeysAccessible calls : Prop :=
-  Forall (fun call => match Blockchain.call_msg call with
-                      | Some (signup public_key) =>
-                        exists secret_key,
-                          mod_pow generator secret_key prime = public_key
-                      | _ => True
-                      end) calls.
-
+Local Open Scope nat.
 Theorem boardroom_voting_correct bstate caddr (trace : ChainTrace empty_state bstate) :
     env_contracts bstate caddr = Some (boardroom_voting : WeakContract) ->
     exists (cstate : State)
@@ -216,10 +246,179 @@ Theorem boardroom_voting_correct bstate caddr (trace : ChainTrace empty_state bs
       deployment_info Setup trace caddr = Some depinfo /\
       contract_state bstate caddr = Some cstate /\
       incoming_calls Msg trace caddr = Some inc_calls /\
-      let Ys := reconstructed_keys (FMap.values (registered_voters cstate)) in
-      SecretKeysAccessible inc_calls ->
-      True.
 
+      finish_registration_by (setup cstate) < finish_vote_by (setup cstate) /\
+      (Blockchain.current_slot bstate < finish_vote_by (setup cstate) ->
+       result cstate = None) /\
+      forall sks svs,
+        SecretsKnown sks svs inc_calls ->
+        (forall addr inf,
+            FMap.find addr (registered_voters cstate) = Some inf ->
+            index inf < length (public_keys cstate) /\
+            nth (index inf) (public_keys cstate) 0%Z = compute_public_key (sks addr)) /\
+        (result cstate = None \/
+         result cstate = Some (sumnat
+                                 (fun party => if svs party then 1 else 0)%nat
+                                 (FMap.keys (registered_voters cstate)))).
+Proof.
+  contract_induction; intros.
+  - split; [tauto|].
+    [AddBlockFacts]: exact (fun _ old_slot _ _ new_slot _ => old_slot < new_slot).
+    subst AddBlockFacts.
+    cbn in facts.
+    split; [destruct IH as [_ [IH _]]|tauto].
+    intros fact.
+    apply IH.
+    lia.
+  - cbn -[Nat.ltb] in *.
+    destruct (_ <? _) eqn:ltb; [|congruence].
+    apply Nat.ltb_lt in ltb.
+    inversion_clear init_some.
+    cbn.
+    setoid_rewrite FMap.find_empty.
+    intuition.
+  - auto.
+  - cbn -[Nat.ltb] in receive_some.
+    destruct msg as [msg|]; cbn -[Nat.ltb] in *; [|congruence].
+    destruct msg.
+    + (* signup *)
+      destruct (_ <? _)%nat eqn:intime in receive_some; cbn -[Nat.ltb] in *; [congruence|].
+      apply Nat.ltb_ge in intime.
+      destruct (FMap.mem _ _) in receive_some; cbn in *; [|congruence].
+      destruct (FMap.mem _ _) in receive_some; cbn in *; [congruence|].
+      destruct (_ =? _)%Z in receive_some; cbn in *; [|congruence].
+      inversion_clear receive_some.
+      cbn.
+      split; [lia|].
+      split; [tauto|].
+      intros.
+      split; [|intuition].
+      intros.
+      destruct (address_eqb_spec addr (ctx_from ctx)) as [->|].
+      * rewrite FMap.find_add in H2.
+        inversion_clear H2.
+        cbn.
+        unfold make_signup_msg in H1.
+        rewrite nth_snoc.
+        rewrite app_length.
+        cbn.
+        split; [lia|].
+        destruct H1; congruence.
+      * rewrite FMap.find_add_ne in H2 by auto.
+        destruct IH as [_ [_ IH]].
+        destruct H1 as [_ H1].
+        specialize (IH sks svs H1).
+        destruct IH as [IH _].
+        specialize (IH _ _ H2).
+        rewrite app_length; split; [lia|].
+        destruct IH.
+        now rewrite app_nth1 by lia.
+    + (* commit_to_vote *)
+
+      split; try tauto.
+
+
+    unfold run_contract_receiver in *.
 End Theories.
 
 End BoardroomVoting.
+(*
+
+Require Import LocalBlockchain.
+
+Fixpoint reconstructed_keys_aux
+        (pks : list Z) (lprod rprod : Z) : list Z :=
+  match pks with
+  | [] => []
+  | pk :: tl =>
+    let rprod := rprod * pk in
+    let rk := lprod * rprod mod modulus in
+    rk :: reconstructed_keys_aux tl (lprod * pk) rprod
+  end.
+
+Definition reconstructed_keys (pks : list Z) : list Z :=
+  let rprod := fold_right (fun e r => (e * r) mod modulus) 1 pks in
+  let rprod := mod_inv rprod modulus in
+  reconstructed_keys_aux pks 1 rprod.
+
+
+Definition modulus : Z := 1552518092300708935130918131258481755631334049434514313202351194902966239949102107258669453876591642442910007680288864229150803718918046342632727613031282983744380820890196288509170691316593175367469551763119843371637221007210577919.
+Definition generator : Z := 2.
+Definition sk n := mod_pow ((Z.of_nat n + 1234583932) * (modulus - 23241)) 159338231 modulus.
+
+Definition num_parties : nat := 7.
+Definition votes_for : nat := 3.
+Definition sks : list Z := Eval native_compute in map sk (seq 7 num_parties).
+Definition pks : list Z := Eval native_compute in map (fun sk => mod_pow generator sk modulus) sks.
+Definition svs : list bool :=
+  Eval compute in map (fun _ => true)
+                      (seq 0 votes_for)
+                  ++ map (fun _ => false)
+                         (seq 0 (num_parties - votes_for)).
+Definition expected_result : nat :=
+  Eval compute in (fold_right (fun (e : bool) r => r + if e then 1 else 0) 0 svs)%nat.
+Definition rks : Vector.t Z (length pks) := Eval native_compute in reconstructed_keys modulus pks.
+Definition pvs : list Z :=
+  Eval native_compute in
+    (fix f (sks : list Z) (rks : list Z) (svs : list bool) :=
+       match sks, rks, svs with
+       | sk :: sks, rk :: rks, sv :: svs =>
+         (mod_pow rk sk modulus * generator^(if sv then 1 else 0)) mod modulus :: f sks rks svs
+       | _, _, _ => []
+       end) sks (Vector.to_list rks) svs.
+
+Definition A a :=
+  BoundedN.of_Z_const AddrSize a.
+
+Local Open Scope nat.
+Definition addrs : list Address.
+Proof.
+  let rec add_addr z n :=
+    match n with
+    | O => constr:(@nil Address)
+    | S ?n => let tail := add_addr (z + 1)%Z n in
+              constr:(cons (A z) tail)
+    end in
+  let num := eval compute in num_parties in
+  let tm := add_addr 11%Z num in
+  let tm := eval vm_compute in tm in
+  exact tm.
+Defined.
+
+Definition deploy_setup :=
+  {| eligible_voters := FMap.of_list (map (fun a => (a, tt)) addrs);
+     finish_registration_by := 3;
+     finish_commit_by := None;
+     finish_vote_by := 5;
+     registration_deposit := 0; |}.
+
+Import Blockchain.
+Definition boardroom_example : option nat :=
+  let chain : LocalChainBuilderDepthFirst := builder_initial in
+  let creator := A 10 in
+  let add_block (chain : LocalChainBuilderDepthFirst) (acts : list Action) :=
+      let next_header :=
+          {| block_height := S (chain_height chain);
+             block_slot := S (current_slot chain);
+             block_finalized_height := finalized_height chain;
+             block_creator := creator;
+             block_reward := 50; |} in
+      builder_add_block chain next_header acts in
+  do chain <- add_block chain [];
+  let dep := build_act creator (create_deployment 0 (boardroom_voting id modulus generator) deploy_setup) in
+  do chain <- add_block chain [dep];
+  do caddr <- hd None (map Some (FMap.keys (lc_contracts (lcb_lc chain))));
+  let reg addr pk := build_act addr (act_call caddr 0 (serialize (signup pk))) in
+  let calls := map (fun '(addr, pk) => reg addr pk) (zip addrs pks) in
+  do chain <- add_block chain calls;
+  let vote addr v := build_act addr (act_call caddr 0 (serialize (submit_vote v))) in
+  let votes := map (fun '(addr, pv) => vote addr pv) (zip addrs pvs) in
+  do chain <- add_block chain votes;
+  do chain <- add_block chain [];
+  let tally := build_act creator (act_call caddr 0 (serialize tally_votes)) in
+  do chain <- add_block chain [tally];
+  do state <- contract_state (lcb_lc chain) caddr;
+  result state.
+
+Eval native_compute in boardroom_example.
+*)
